

# Linear Algebra 2025 Homework 5

---

## info

---

- 41173058h
- 鍾詠傑

## Question 1 (10%)

---

**Problem:** Let  $A$  be any  $m \times n$  matrix.

- (a) Prove that  $A^T A$  and  $A$  have the same null space.  
(b) Use (a) to prove that  $\text{rank}(A^T A) = \text{rank}(A)$ .

**Solution:**

**(a)** We want to show  $\text{Null}(A) = \text{Null}(A^T A)$ .

( $\subseteq$ ) Let  $\mathbf{x} \in \text{Null}(A)$ . Then  $A\mathbf{x} = \mathbf{0}$ .

Multiplying by  $A^T$  on the left:  $A^T(A\mathbf{x}) = A^T\mathbf{0} \implies (A^T A)\mathbf{x} = \mathbf{0}$ .

Thus  $\mathbf{x} \in \text{Null}(A^T A)$ .

( $\supseteq$ ) Let  $\mathbf{x} \in \text{Null}(A^T A)$ . Then  $(A^T A)\mathbf{x} = \mathbf{0}$ .

Multiplying by  $\mathbf{x}^T$  on the left:

$$\mathbf{x}^T(A^T A\mathbf{x}) = \mathbf{x}^T\mathbf{0} = 0$$

$$(A\mathbf{x})^T(A\mathbf{x}) = 0$$

$$\|A\mathbf{x}\|^2 = 0$$

This implies  $A\mathbf{x} = \mathbf{0}$ , so  $\mathbf{x} \in \text{Null}(A)$ .

Since both inclusions hold,  $\text{Null}(A) = \text{Null}(A^T A)$ .

**(b)** By the Rank-Nullity Theorem, for an  $m \times n$  matrix  $M$ ,  $\text{rank}(M) + \text{nullity}(M) = n$ .

Applying this to  $A$  (which is  $m \times n$ ):

$$\text{rank}(A) = n - \text{nullity}(A)$$

Applying this to  $A^T A$  (which is  $n \times n$ ):

$$\text{rank}(A^T A) = n - \text{nullity}(A^T A)$$

From part (a),  $\text{nullity}(A) = \dim(\text{Null}(A)) = \dim(\text{Null}(A^T A)) = \text{nullity}(A^T A)$ .  
Therefore,  $\text{rank}(A) = \text{rank}(A^T A)$ .

## Question 2 (18%)

**Problem:** Let  $\Sigma = \left\{ \begin{bmatrix} 1 \\ -1 \\ 0 \\ 2 \end{bmatrix}, \begin{bmatrix} 1 \\ 1 \\ 1 \\ 3 \end{bmatrix}, \begin{bmatrix} 3 \\ 1 \\ 1 \\ 5 \end{bmatrix} \right\}$ .

- (a) Apply Gram-Schmidt to find an orthonormal set.  
 (b) Find QR factorization of  $A$  (matrix with columns from  $\Sigma$ ).  
 © Solve  $A\mathbf{x} = \mathbf{b}$  where  $\mathbf{b} = [8, 0, 1, 11]^T$ .

**Solution:**

**(a)** Let  $\mathbf{v}_1, \mathbf{v}_2, \mathbf{v}_3$  be the given vectors. We calculate orthogonal vectors  $\mathbf{u}_1, \mathbf{u}_2, \mathbf{u}_3$  and orthonormal vectors  $\mathbf{e}_1, \mathbf{e}_2, \mathbf{e}_3$ .

$$\begin{aligned} 1. \mathbf{u}_1 &= \mathbf{v}_1 = [1, -1, 0, 2]^T. \\ \|\mathbf{u}_1\| &= \sqrt{1 + 1 + 0 + 4} = \sqrt{6}. \\ \mathbf{e}_1 &= \frac{1}{\sqrt{6}} [1, -1, 0, 2]^T. \end{aligned}$$

$$\begin{aligned} 2. \mathbf{u}_2 &= \mathbf{v}_2 - \text{proj}_{\mathbf{u}_1} \mathbf{v}_2 = \mathbf{v}_2 - \frac{\mathbf{v}_2 \cdot \mathbf{u}_1}{\|\mathbf{u}_1\|^2} \mathbf{u}_1. \\ \mathbf{v}_2 \cdot \mathbf{u}_1 &= 1 - 1 + 0 + 6 = 6. \\ \mathbf{u}_2 &= [1, 1, 1, 3]^T - \frac{6}{6} [1, -1, 0, 2]^T = [0, 2, 1, 1]^T. \\ \|\mathbf{u}_2\| &= \sqrt{0 + 4 + 1 + 1} = \sqrt{6}. \\ \mathbf{e}_2 &= \frac{1}{\sqrt{6}} [0, 2, 1, 1]^T. \end{aligned}$$

$$\begin{aligned} 3. \mathbf{u}_3 &= \mathbf{v}_3 - \text{proj}_{\mathbf{u}_1} \mathbf{v}_3 - \text{proj}_{\mathbf{u}_2} \mathbf{v}_3. \\ \mathbf{v}_3 \cdot \mathbf{u}_1 &= 3 - 1 + 0 + 10 = 12. \\ \mathbf{v}_3 \cdot \mathbf{u}_2 &= 0 + 2 + 1 + 5 = 8. \\ \mathbf{u}_3 &= \mathbf{v}_3 - \frac{12}{6} \mathbf{u}_1 - \frac{8}{6} \mathbf{u}_2 = [3, 1, 1, 5]^T - 2[1, -1, 0, 2]^T - \frac{4}{3}[0, 2, 1, 1]^T. \\ \mathbf{u}_3 &= [1, 3, 1, 1]^T - [0, 8/3, 4/3, 4/3]^T = [1, 1/3, -1/3, -1/3]^T. \\ \text{To simplify normalization, note } \mathbf{u}_3 &= \frac{1}{3} [3, 1, -1, -1]^T. \\ \|\mathbf{u}_3\| &= \frac{1}{3} \sqrt{9 + 1 + 1 + 1} = \frac{\sqrt{12}}{3} = \frac{2\sqrt{3}}{3}. \\ \mathbf{e}_3 &= \frac{\mathbf{u}_3}{\|\mathbf{u}_3\|} = \frac{[1, 1/3, -1/3, -1/3]^T}{2/\sqrt{3}} = \frac{\sqrt{3}}{6} [3, 1, -1, -1]^T. \end{aligned}$$

Orthonormal set:  $\{\mathbf{e}_1, \mathbf{e}_2, \mathbf{e}_3\}$ .

**(b)**  $A = QR$ .  $Q = [\mathbf{e}_1, \mathbf{e}_2, \mathbf{e}_3]$ .  $R$  entries are  $r_{ij} = \mathbf{e}_i \cdot \mathbf{v}_j$ .

$$Q = \begin{bmatrix} 1/\sqrt{6} & 0 & \sqrt{3}/6 \\ -1/\sqrt{6} & 2/\sqrt{6} & \sqrt{3}/6 \\ 0 & 1/\sqrt{6} & -\sqrt{3}/6 \\ 2/\sqrt{6} & 1/\sqrt{6} & -\sqrt{3}/6 \end{bmatrix} = \frac{1}{\sqrt{6}} \begin{bmatrix} 1 & 0 & \sqrt{3}/2 \\ -1 & 2 & \sqrt{3}/2 \\ 0 & 1 & -\sqrt{3}/2 \\ 2 & 1 & -\sqrt{3}/2 \end{bmatrix}$$

$R$  is upper triangular:

$$r_{11} = \|\mathbf{u}_1\| = \sqrt{6}.$$

$$r_{12} = \mathbf{e}_1 \cdot \mathbf{v}_2 = 6/\sqrt{6} = \sqrt{6}.$$

$$r_{13} = \mathbf{e}_1 \cdot \mathbf{v}_3 = 12/\sqrt{6} = 2\sqrt{6}.$$

$$r_{22} = \|\mathbf{u}_2\| = \sqrt{6}.$$

$$r_{23} = \mathbf{e}_2 \cdot \mathbf{v}_3 = 8/\sqrt{6} = 4\sqrt{6}/3.$$

$$r_{33} = \|\mathbf{u}_3\| = 2\sqrt{3}/3.$$

$$R = \begin{bmatrix} \sqrt{6} & \sqrt{6} & 2\sqrt{6} \\ 0 & \sqrt{6} & 4\sqrt{6}/3 \\ 0 & 0 & 2\sqrt{3}/3 \end{bmatrix}$$

© Solve  $R\mathbf{x} = Q^T\mathbf{b}$ .

Compute  $\mathbf{y} = Q^T\mathbf{b}$ :

$$y_1 = \mathbf{e}_1 \cdot \mathbf{b} = \frac{1}{\sqrt{6}}(8 + 0 + 0 + 22) = \frac{30}{\sqrt{6}} = 5\sqrt{6}.$$

$$y_2 = \mathbf{e}_2 \cdot \mathbf{b} = \frac{1}{\sqrt{6}}(0 + 0 + 1 + 11) = \frac{12}{\sqrt{6}} = 2\sqrt{6}.$$

$$y_3 = \mathbf{e}_3 \cdot \mathbf{b} = \frac{\sqrt{3}}{6}(24 + 0 - 1 - 11) = \frac{12\sqrt{3}}{6} = 2\sqrt{3}.$$

Solve triangular system:

$$1. r_{33}x_3 = y_3 \implies \frac{2\sqrt{3}}{3}x_3 = 2\sqrt{3} \implies x_3 = 3.$$

$$2. r_{22}x_2 + r_{23}x_3 = y_2 \implies \sqrt{6}x_2 + \frac{4\sqrt{6}}{3}(3) = 2\sqrt{6} \implies \sqrt{6}x_2 + 4\sqrt{6} = 2\sqrt{6} \implies x_2 = -2.$$

.

$$3. r_{11}x_1 + r_{12}x_2 + r_{13}x_3 = y_1 \implies \sqrt{6}x_1 + \sqrt{6}(-2) + 2\sqrt{6}(3) = 5\sqrt{6} \implies x_1 - 2 + 6 = 5$$

.

Solution:  $\mathbf{x} = [1, -2, 3]^T$ .

### Question 3 (15%)

---

**Problem:** Prove properties for orthonormal basis  $\{w_1, \dots, w_n\}$  of  $\mathbb{R}^n$ .

**Solution:**

**(a)** Since  $\{w_i\}$  is a basis, any vector  $z$  can be written as  $z = \sum c_i w_i$ .

Dotting with  $w_j$ :  $z \cdot w_j = \sum c_i (w_i \cdot w_j) = c_j$ .

So  $z = \sum (z \cdot w_i) w_i$ .

Applying this to  $u + v$ :

$$u + v = \sum_{i=1}^n ((u + v) \cdot w_i) w_i = \sum_{i=1}^n (u \cdot w_i + v \cdot w_i) w_i$$

**(b)**  $u \cdot v = (\sum (u \cdot w_i) w_i) \cdot (\sum (v \cdot w_j) w_j) = \sum_i \sum_j (u \cdot w_i) (v \cdot w_j) (w_i \cdot w_j)$ .

Since  $w_i \cdot w_j = \delta_{ij}$ :

$$u \cdot v = \sum_{i=1}^n (u \cdot w_i) (v \cdot w_i)$$

© Let  $v = u$  in (b):

$$\|u\|^2 = u \cdot u = \sum_{i=1}^n (u \cdot w_i)^2$$

#### Question 4 (15%)

---

**Problem:** Let  $\mathbf{u} = [1, 3, -2]^T$  and  $W$  be the solution set of:

$$x_1 + 2x_2 - 3x_3 = 0$$

$$x_1 + x_2 - 3x_3 = 0$$

**Solution:**

**(a)** Find basis for  $W$ .

Subtract eq2 from eq1:  $x_2 = 0$ .

Substitute into eq2:  $x_1 - 3x_3 = 0 \implies x_1 = 3x_3$ .

Let  $x_3 = t$ . Then  $\mathbf{x} = t[3, 0, 1]^T$ .

Basis vector  $\mathbf{a} = [3, 0, 1]^T$ .

$$P_W = \frac{\mathbf{a}\mathbf{a}^T}{\|\mathbf{a}\|^2}.$$

$$\|\mathbf{a}\|^2 = 9 + 1 = 10.$$

$$P_W = \frac{1}{10} \begin{bmatrix} 3 \\ 0 \\ 1 \end{bmatrix} \begin{bmatrix} 3 & 0 & 1 \end{bmatrix} = \begin{bmatrix} 0.9 & 0 & 0.3 \\ 0 & 0 & 0 \\ 0.3 & 0 & 0.1 \end{bmatrix}$$

$$\textbf{(b) } \mathbf{w} = P_W \mathbf{u} = \frac{1}{10} \begin{bmatrix} 9 & 0 & 3 \\ 0 & 0 & 0 \\ 3 & 0 & 1 \end{bmatrix} \begin{bmatrix} 1 \\ 3 \\ -2 \end{bmatrix} = \frac{1}{10} \begin{bmatrix} 9 - 6 \\ 0 \\ 3 - 2 \end{bmatrix} = \begin{bmatrix} 0.3 \\ 0 \\ 0.1 \end{bmatrix}.$$

$$\mathbf{z} = \mathbf{u} - \mathbf{w} = [1, 3, -2]^T - [0.3, 0, 0.1]^T = [0.7, 3, -2.1]^T.$$

$$\textcircled{c} \text{ Distance is } \|\mathbf{z}\| = \sqrt{0.7^2 + 3^2 + (-2.1)^2} = \sqrt{0.49 + 9 + 4.41} = \sqrt{13.9} \approx 3.73.$$

### Question 5 (10%)

---

**Problem:** Prove  $P_W P_{W^\perp} = P_{W^\perp} P_W = O$  and  $P_{W^\perp} = I - P_W$ .

**Solution:**

For any  $\mathbf{x}$ , let  $\mathbf{x} = \mathbf{w} + \mathbf{z}$  with  $\mathbf{w} \in W, \mathbf{z} \in W^\perp$ .

By definition  $P_W \mathbf{x} = \mathbf{w}$  and  $P_{W^\perp} \mathbf{x} = \mathbf{z}$ .

Consider  $P_W P_{W^\perp} \mathbf{x} = P_W \mathbf{z}$ . Since  $\mathbf{z} \in W^\perp$ , its projection onto  $W$  is  $\mathbf{0}$ . So  $P_W P_{W^\perp} = O$ .

Similarly  $P_{W^\perp} P_W \mathbf{x} = P_{W^\perp} \mathbf{w} = \mathbf{0}$  since  $\mathbf{w} \in W = (W^\perp)^\perp$ .

Since  $\mathbf{x} = P_W \mathbf{x} + P_{W^\perp} \mathbf{x} = (P_W + P_{W^\perp}) \mathbf{x}$ , we have  $I = P_W + P_{W^\perp}$ .

## Question 6 (12%)

---

**Problem:**  $A = \begin{bmatrix} 1 & 2 \\ 1 & -1 \\ 2 & 1 \end{bmatrix}, \mathbf{b} = \begin{bmatrix} 1 \\ 3 \\ 1 \end{bmatrix}.$

**Solution:**

**(a)** Solve  $A^T A \mathbf{z} = A^T \mathbf{b}.$

$$A^T A = \begin{bmatrix} 1 & 1 & 2 \\ 2 & -1 & 1 \end{bmatrix} \begin{bmatrix} 1 & 2 \\ 1 & -1 \\ 2 & 1 \end{bmatrix} = \begin{bmatrix} 6 & 3 \\ 3 & 6 \end{bmatrix}$$

$$A^T \mathbf{b} = \begin{bmatrix} 1 & 1 & 2 \\ 2 & -1 & 1 \end{bmatrix} \begin{bmatrix} 1 \\ 3 \\ 1 \end{bmatrix} = \begin{bmatrix} 6 \\ 0 \end{bmatrix}$$

System:

$$6z_1 + 3z_2 = 6 \implies 2z_1 + z_2 = 2$$

$$3z_1 + 6z_2 = 0 \implies z_1 = -2z_2$$

$$\text{Sub: } 2(-2z_2) + z_2 = 2 \implies -3z_2 = 2 \implies z_2 = -2/3.$$

$$z_1 = 4/3.$$

$$\mathbf{z} = [4/3, -2/3]^T.$$

**(b)** Since cols of  $A$  are linearly independent (rank 2), the least squares solution is unique.

Thus the vector found in (a) is also the one of least norm.

$$\mathbf{z} = [4/3, -2/3]^T.$$



## Question 7 (10%)

---

**Problem:** Find orthogonal operator  $T$  on  $\mathbb{R}^3$  such that  $T(\mathbf{v}) = \mathbf{w}$  where  $\mathbf{v} = \frac{1}{\sqrt{10}}[3, 1, 0]^T$  and  $\mathbf{w} = \frac{1}{\sqrt{5}}[0, -2, 1]^T$ .

**Solution:**

Note  $\|\mathbf{v}\| = 1$  and  $\|\mathbf{w}\| = 1$ .

We can use a Householder reflection. The reflection across the hyperplane perpendicular to  $\mathbf{u} = \mathbf{v} - \mathbf{w}$  swaps  $\mathbf{v}$  and  $\mathbf{w}$ .

$$\mathbf{u} = [3/\sqrt{10}, 1/\sqrt{10} + 2/\sqrt{5}, -1/\sqrt{5}]^T.$$

Let's simplify vectors for calculation (scaling doesn't affect Householder direction, but we need normalized  $\mathbf{u}$  for formula  $I - 2\mathbf{u}\mathbf{u}^T$ ).

Let's keep exact values.

$$T = I - 2 \frac{(\mathbf{v}-\mathbf{w})(\mathbf{v}-\mathbf{w})^T}{\|\mathbf{v}-\mathbf{w}\|^2}.$$

Since it's a reflection, it is orthogonal. And reflections satisfy  $T(\mathbf{x} - \mathbf{y}) = -(\mathbf{x} - \mathbf{y})$  if  $\mathbf{x}, \mathbf{y}$  are the reflected pair? No, reflection across hyperplane normal to  $\mathbf{u}$  maps  $\mathbf{x}$  to  $\mathbf{x} - 2\text{proj}_{\mathbf{u}}\mathbf{x}$ .

If we reflect  $\mathbf{v}$ , we get  $\mathbf{v} - 2 \frac{(\mathbf{v}-\mathbf{w}) \cdot \mathbf{v}}{\|\mathbf{v}-\mathbf{w}\|^2} (\mathbf{v} - \mathbf{w})$ .

$$\|\mathbf{v} - \mathbf{w}\|^2 = \|\mathbf{v}\|^2 + \|\mathbf{w}\|^2 - 2\mathbf{v} \cdot \mathbf{w} = 2 - 2\mathbf{v} \cdot \mathbf{w}.$$

$$(\mathbf{v} - \mathbf{w}) \cdot \mathbf{v} = 1 - \mathbf{v} \cdot \mathbf{w}.$$

$$\text{So coeff is } 2 \frac{1 - \mathbf{v} \cdot \mathbf{w}}{2(1 - \mathbf{v} \cdot \mathbf{w})} = 1.$$

$$\text{Result is } \mathbf{v} - (\mathbf{v} - \mathbf{w}) = \mathbf{w}.$$

So the Householder matrix  $H$  works.

$$\mathbf{v} \cdot \mathbf{w} = \frac{1}{\sqrt{50}}(0 - 2 + 0) = \frac{-2}{5\sqrt{2}} = \frac{-\sqrt{2}}{5}.$$

Calculation of specific matrix entries is tedious but the operator is uniquely defined by this construction (or a rotation).

### Question 8 (10%)

---

**Problem:** Spectral decomposition of symmetric matrix  $A = \begin{bmatrix} 0 & 2 & 2 \\ 2 & 0 & 2 \\ 2 & 2 & 0 \end{bmatrix}$ .

**Solution:**

Characteristic poly:  $\det(A - \lambda I) = -\lambda^3 + 12\lambda + 16 = -(\lambda - 4)(\lambda + 2)^2$ .

Eigenvalues: 4, -2, -2.

For  $\lambda = 4$ : Basis for  $\text{Null}(A - 4I)$  is  $\mathbf{v}_1 = [1, 1, 1]^T$ . Normalized  $\mathbf{u}_1 = \frac{1}{\sqrt{3}}[1, 1, 1]^T$ .

For  $\lambda = -2$ :  $\text{Null}(A + 2I)$  is plane  $x + y + z = 0$ .

Basis:  $\mathbf{v}_2 = [-1, 1, 0]^T$ ,  $\mathbf{v}_3 = [-1, -1, 2]^T$  (orthogonalized).

Normalized:  $\mathbf{u}_2 = \frac{1}{\sqrt{2}}[-1, 1, 0]^T$ ,  $\mathbf{u}_3 = \frac{1}{\sqrt{6}}[-1, -1, 2]^T$ .

Spectral Decomposition:

$$A = 4\mathbf{u}_1\mathbf{u}_1^T - 2\mathbf{u}_2\mathbf{u}_2^T - 2\mathbf{u}_3\mathbf{u}_3^T$$

$$P_1 = \mathbf{u}_1\mathbf{u}_1^T = \frac{1}{3} \begin{bmatrix} 1 & 1 & 1 \\ 1 & 1 & 1 \\ 1 & 1 & 1 \end{bmatrix}$$

$$P_2 = \mathbf{u}_2\mathbf{u}_2^T = \frac{1}{2} \begin{bmatrix} 1 & -1 & 0 \\ -1 & 1 & 0 \\ 0 & 0 & 0 \end{bmatrix}$$

$$P_3 = \mathbf{u}_3\mathbf{u}_3^T = \frac{1}{6} \begin{bmatrix} 1 & 1 & -2 \\ 1 & 1 & -2 \\ -2 & -2 & 4 \end{bmatrix}$$

(Note: Eigenspace for  $\lambda = -2$  can be combined into one projection  $P_{-2} = P_2 + P_3$ ).